adding bytes

src/RIoTCore.fst
@@ -1,15 +1,30 @@
 module RIoTCore
 
-open FStar.Buffer
-open FStar.UInt32
 
 module HS  = FStar.HyperStack
-module B   = FStar.Buffer
+module HST = FStar.HyperStack.ST
+module B   = LowStar.Buffer
+module M   = LowStar.Modifies
+module U64 = FStar.UInt64
 module U32 = FStar.UInt32
+module U16 = FStar.UInt16
 module U8  = FStar.UInt8
+module Bytes = FStar.Bytes
 
+let uint64 = U64.t
 let uint32 = U32.t
-let uint8 = U8.t
+let uint16 = U16.t
+let uint8  = U8.t
+let bytes   = Bytes.bytes
+
+let _DICE_UDS_LENGTH    : U32.t = 0x20ul
+let _DICE_DIGEST_LENGTH : U32.t = 0x20ul
+
+let _UDS = B.malloca_of_list [0;1]
+
+let _DEFAULT_RIOT_PATH : string = "riot.dll"
+let _DEFAULT_LOADER_PATH : string = "FW.dll"
+let _RIOT_ENTRY : string = "RiotStart"
 
 // TODO: Date Types
 // TODO: Modules
@@ -34,119 +49,13 @@ effect ST
 
 effect St (a:Type) = FStar.HyperStack.ST.St a
 
-val _DICEStart (something:unit) : ST unit
+val _DICEStart
+  (riotImagePath   : string)
+  (loaderImagePath : string)
+: ST unit
   (requires fun h -> True)
   (ensures  fun h0 _ h1 -> True)
-let _DICEStart () = ()
-let a = _DICEStart ()
-(*
-let _RiotStart (_CDI:string) (_CDILen:nat) =
-  // DONE: Get CDI Digest
-  // REF: RiotCrypt_Hash(cDigest, RIOT_DIGEST_LENGTH, CDI, CDILen);
-  // NOTE: pointer in F*?
-  let cDigest = (_RiotCrypt_Hash _RIOT_DIGEST_LENGTH
-                                 _CDI // <--
-                                 _CDILen) in
-
-  // DONE: Derive DeviceID Key pair
-  // REF: RiotCrypt_DeriveEccKey(&DeviceIDPub,
-  //                             &deviceIDPriv,
-  //                             cDigest, RIOT_DIGEST_LENGTH,
-  //                             (const uint8_t * )RIOT_LABEL_IDENTITY,
-  //                             lblSize(RIOT_LABEL_IDENTITY));
-  // NOTE: F* represents a record (inductive type) in a form of product type?
-  let (_DeviceIDPub, _DeviceIDPriv) =
-                     (_RiotCrypt_DeriveEccKey cDigest // <--
-                                              _RIOT_DIGEST_LENGTH
-                                              _RIOT_LABEL_IDENTITY
-                                              _RIOT_LABEL_IDENTITY_SIZE) in
-
-  // TODO: Set the serial number for DeviceID certificate
-  // REF: RiotSetSerialNumber(&x509DeviceTBSData, cDigest, RIOT_DIGEST_LENGTH);
-
-  // TODO: Output Device Identity Key pair
-  // REF:
-
-  // TODO: Locate firmware image
-  // REF: fwDLL = LoadLibrary(FWImagePath);
-  //      if (fwDLL == NULL) {
-  //          printf("RIOT: ERROR: Failed to load firmware image.\n");
-  //          return;
-  //      }
-
-  // TODO: Locate entry point for FW
-  // REF: FirmwareEntry = (fpFirmwareEntry)GetProcAddress(fwDLL, FIRMWARE_ENTRY);
-  //      if (!FirmwareEntry) {
-  //          printf("RIOT: ERROR: Failed to locate fw start\n");
-  //          return;
-  //      }
-
-  // TODO: Get base offset and size of FW image
-  // REF: if (!RiotGetFWInfo(fwDLL, &offset, &fwSize)) {
-  //          fprintf(stderr, "FW: Failed to locate FW code\n");
-  //          return;
-  //      }
-
-  // TODO: Calculate base VA of FW code
-  // REF: fwImage = (BYTE *)((uint64_t)fwDLL + offset);
-
-  // DONE: Measure FW, i.e., calculate FWID
-  // REF: RiotCrypt_Hash(FWID, RIOT_DIGEST_LENGTH, fwImage, fwSize);
-  let _FWID = (_RiotCrypt_Hash _RIOT_DIGEST_LENGTH
-                               _fwImage // <--
-                               _fwSize) in
-
-  // DONE: Combine CDI and FWID, result in cDigest
-  // REF: RiotCrypt_Hash2(cDigest, RIOT_DIGEST_LENGTH,
-  //       cDigest, RIOT_DIGEST_LENGTH,
-  //       FWID,    RIOT_DIGEST_LENGTH);
-  let cDigest = (_RiotCrypt_Hash2 _RIOT_DIGEST_LENGTH
-                                  cDigest // <--
-                                  _RIOT_DIGEST_LENGTH
-                                  _FWID // <--
-                                  _RIOT_DIGEST_LENGTH) in
-
-  // DONE: Derive Alias key pair from CDI and FWID
-  // REF: RiotCrypt_DeriveEccKey(&AliasKeyPub,
-  //                             &AliasKeyPriv,
-  //                             cDigest, RIOT_DIGEST_LENGTH,
-  //                             (const uint8_t *)RIOT_LABEL_ALIAS,
-  //                             lblSize(RIOT_LABEL_ALIAS));
-  let (_AliasKeyPub, _AliasKeyPriv) = (_RiotCrypt_DeriveEccKey cDigest // <--
-                                                               _RIOT_DIGEST_LENGTH
-                                                               _RIOT_LABEL_IDENTITY
-                                                               _RIOT_LABEL_IDENTITY_SIZE) in
-
-  // TODO: With the Alias Key pair derived, we can now Seed DRBG
-  // REF: RiotCrypt_SeedDRBG((uint8_t*)&AliasKeyPriv, sizeof(RIOT_ECC_PRIVATE));
-  // NOTE: DRBG for Deterministic Random Bit Generator?
-
-  // TODO: Set the serial number
-  // REF: RiotSetSerialNumber(&x509AliasTBSData, cDigest, RIOT_DIGEST_LENGTH);
-
-  // TODO: Clean up potentially sensative data
-  // REF: memset(cDigest, 0x00, RIOT_DIGEST_LENGTH);
-  // NOTE: Does F* supports memory operation?
-
-  // TODO: Build the TBS (to be signed) region of Alias Key Certificate
-  // REF: DERInitContext(&derCtx, derBuffer, DER_MAX_TBS);
-  //      X509GetAliasCertTBS(&derCtx, &x509AliasTBSData,
-  //                          &AliasKeyPub, &DeviceIDPub,
-  //                          FWID, RIOT_DIGEST_LENGTH);
-
-  // TODO: Sign the Alias Key Certificate's TBS region
-  // REF: RiotCrypt_Sign(&tbsSig, derCtx.Buffer, derCtx.Position, &deviceIDPriv);
-  //let tbsSig = (_RiotCrypt_Sign derCtx.Buffer
-  //                              derCtx.Position
-  //                              deviceIDPriv) in
-
-  // TODO: Generate Alias Key Certificate
-  // REF: X509MakeAliasCert(&derCtx, &tbsSig);
-
-  // TODO: Copy Alias Key Certificate
-  // REF: length = sizeof(AliasCert);
-  //      DERtoPEM(&derCtx, CERT_TYPE, AliasCert, &length);
-  //      AliasCert[length] = '\0';
-
-false
-*)
+let _DICEStart _ =
+  let uDigest = B.malloc HS.root 0ul _DICE_DIGEST_LENGTH in
+  let rDigest = B.malloc HS.root 0ul _DICE_DIGEST_LENGTH in
+  ()
